combinators

src/lowparse/steel_st_array/LowParse.SteelST.Access.fst
@@ -6,14 +6,14 @@ module SZ = LowParse.Steel.StdInt
 
 open Steel.ST.Util
 
-let parsed_size
+let jumper
   (#k: parser_kind)
   (#t: Type)
   (p: parser k t)
 : Tot (Type u#1)
 =
-  (base: Type) ->
-  (va: AP.v base byte) ->
+  (#base: Type) ->
+  (#va: AP.v base byte) ->
   (a: byte_array base) ->
   ST SZ.size_t
     (AP.arrayptr a va)
@@ -26,19 +26,19 @@ let parsed_size
         SZ.size_v res == consumed
 )
 
-let parsed_size_constant_size
+let jump_constant_size
   (#k: parser_kind)
   (#t: Type)
   (p: parser k t)
   (sz: SZ.size_t)
-: Pure (parsed_size p)
+: Pure (jumper p)
     (requires (
       k.parser_kind_high == Some k.parser_kind_low /\
       SZ.size_v sz == k.parser_kind_low
     ))
     (ensures (fun _ -> True))
 =
-  fun base va a ->
+  fun #base #va a ->
   parser_kind_prop_equiv k p;
   noop ();
   return sz
@@ -49,7 +49,7 @@ let get_parsed_size
   (#t: Type)
   (#p: parser k t)
   (#vp: v base k t)
-  (j: parsed_size p)
+  (j: jumper p)
   (a: byte_array base)
 : ST SZ.size_t
     (aparse p a vp)
@@ -58,7 +58,7 @@ let get_parsed_size
     (fun res -> SZ.size_v res == AP.length (array_of vp))
 =
   let _ = elim_aparse p a in
-  let res = j base _ a in
+  let res = j a in
   let _ = intro_aparse p a in
   return res
 
@@ -74,81 +74,35 @@ let parse'
 
 #set-options "--ide_id_info_off"
 
-let peek_strong_with_size1
+let ghost_peek_strong
+  (#opened: _)
   (#base: Type)
   (#k: parser_kind)
   (#t: Type)
   (#va: AP.v base byte)
   (p: parser k t)
   (a: byte_array base)
-  (sz: SZ.size_t)
-: ST (byte_array base)
+: STGhost (Ghost.erased (byte_array base)) opened
     (AP.arrayptr a va)
-    (fun res -> exists_ (fun vp -> aparse p a vp `star` exists_ (fun vres -> AP.arrayptr res vres  (* `star` pure (
-True      let consumed = AP.length (array_of vp) in
+    (fun res -> exists_ (fun vp -> aparse p a vp `star` exists_ (fun vres -> AP.arrayptr res vres `star` pure (
+      let consumed = AP.length (array_of vp) in
       AP.merge_into (array_of vp) (AP.array_of vres) (AP.array_of va) /\
       consumed <= AP.length (AP.array_of va) /\
       AP.contents_of' vres == AP.seq_slice (AP.contents_of' va) consumed (AP.length (AP.array_of va)) /\
+      parse' p (AP.contents_of' va) == Some (vp.contents, consumed) /\
       parse' p (AP.seq_slice (AP.contents_of' va) 0 consumed) == Some (vp.contents, consumed)
-    ) *) )  ))
+    )) )  )
     (k.parser_kind_subkind == Some ParserStrong /\
-      begin match parse' p (AP.contents_of' va) with
-      | None -> False
-      | Some (_, consumed) -> (consumed <: nat) == SZ.size_v sz
-      end
+    Some? (parse' p (AP.contents_of' va))
     )
     (fun _ -> True)
 =
-  noop ();
-//  assert (SZ.size_v sz <= Seq.length (AP.contents_of' va));
+  let sz = SZ.int_to_size_t (snd (Some?.v (parse' p (AP.contents_of' va))) <: nat) in
   parse_strong_prefix p (AP.contents_of' va) (AP.seq_slice (AP.contents_of' va) 0 (SZ.size_v sz));
-  let res = AP.split a sz in
-  let _ = elim_exists () in
-  let _ = elim_exists () in
-  let _ = elim_pure _ in
-  noop ();
-  let _ = intro_aparse p a in
-  let vres = vpattern_replace (fun vres -> AP.arrayptr res vres) in
-//  drop (AP.arrayptr res vres);
-  noop ();
-  return res
-
-let peek_strong_with_size2
-  (#base: Type)
-  (#k: parser_kind)
-  (#t: Type)
-  (#va: AP.v base byte)
-  (p: parser k t)
-  (a: byte_array base)
-  (sz: SZ.size_t)
-: ST (byte_array base)
-    (AP.arrayptr a va)
-    (fun res -> exists_ (fun vp -> aparse p a vp `star` exists_ (fun vres -> AP.arrayptr res vres  (* `star` pure (
-True      let consumed = AP.length (array_of vp) in
-      AP.merge_into (array_of vp) (AP.array_of vres) (AP.array_of va) /\
-      consumed <= AP.length (AP.array_of va) /\
-      AP.contents_of' vres == AP.seq_slice (AP.contents_of' va) consumed (AP.length (AP.array_of va)) /\
-      parse' p (AP.seq_slice (AP.contents_of' va) 0 consumed) == Some (vp.contents, consumed)
-    ) *) )  ))
-    (k.parser_kind_subkind == Some ParserStrong /\
-      begin match parse' p (AP.contents_of' va) with
-      | None -> False
-      | Some (_, consumed) -> (consumed <: nat) == SZ.size_v sz
-      end
-    )
-    (fun _ -> True)
-=
-  noop ();
-  assert (SZ.size_v sz <= Seq.length (AP.contents_of' va));
-  parse_strong_prefix p (AP.contents_of' va) (AP.seq_slice (AP.contents_of' va) 0 (SZ.size_v sz));
-  let res = AP.split a sz in
+  let res = AP.gsplit a sz in
   let _ = gen_elim () in
-  noop ();
   let _ = intro_aparse p a in
-  let vres = vpattern_replace (fun vres -> AP.arrayptr res vres) in
-  intro_exists _ (fun vres -> AP.arrayptr res vres);
-  noop ();
-  return res
+  res
 
 let peek_strong_with_size
   (#base: Type)
@@ -164,7 +118,9 @@ let peek_strong_with_size
       let consumed = AP.length (array_of vp) in
       AP.merge_into (array_of vp) (AP.array_of vres) (AP.array_of va) /\
       consumed <= AP.length (AP.array_of va) /\
+      consumed == SZ.size_v sz /\
       AP.contents_of' vres == AP.seq_slice (AP.contents_of' va) consumed (AP.length (AP.array_of va)) /\
+      parse' p (AP.contents_of' va) == Some (vp.contents, consumed) /\
       parse' p (AP.seq_slice (AP.contents_of' va) 0 consumed) == Some (vp.contents, consumed)
     )) )  )
     (k.parser_kind_subkind == Some ParserStrong /\
@@ -174,15 +130,11 @@ let peek_strong_with_size
       end
     )
     (fun _ -> True)
-=
-  noop ();
-  assert (SZ.size_v sz <= Seq.length (AP.contents_of' va));
-  parse_strong_prefix p (AP.contents_of' va) (AP.seq_slice (AP.contents_of' va) 0 (SZ.size_v sz));
-  let res = AP.split a sz in
+= let gres = ghost_peek_strong p a in
   let _ = gen_elim () in
-  noop ();
-  let _ = intro_aparse p a in
-  noop ();
+  let _ = elim_aparse _ a in
+  let res = AP.split' a sz gres in
+  let _ = intro_aparse _ a in
   return res
 
 let peek_strong
@@ -191,7 +143,7 @@ let peek_strong
   (#t: Type)
   (#p: parser k t)
   (#va: AP.v base byte)
-  (j: parsed_size p)
+  (j: jumper p)
   (a: byte_array base)
 : ST (byte_array base)
     (AP.arrayptr a va)
@@ -200,19 +152,20 @@ let peek_strong
       AP.merge_into (array_of vp) (AP.array_of vres) (AP.array_of va) /\
       consumed <= AP.length (AP.array_of va) /\
       AP.contents_of' vres == AP.seq_slice (AP.contents_of' va) consumed (AP.length (AP.array_of va)) /\
+      parse' p (AP.contents_of' va) == Some (vp.contents, consumed) /\
       parse' p (AP.seq_slice (AP.contents_of' va) 0 consumed) == Some (vp.contents, consumed)
     ))))
     (k.parser_kind_subkind == Some ParserStrong /\
       Some? (parse p (AP.contents_of' va)))
     (fun _ -> True)
 =
-  let sz = j base _ a in
+  let sz = j a in
   let res = peek_strong_with_size p a sz in
-  noop ();
+  let _ = gen_elim () in
   return res
 
 /// useful for validators, which need to roll back peek after reading some contents
-let unpeek_strong
+let unpeek_strong'
   (#opened: _)
   (#base: Type)
   (#k: parser_kind)
@@ -244,6 +197,37 @@ let unpeek_strong
   noop ();
   va
 
+let unpeek_strong
+  (#opened: _)
+  (#base: Type)
+  (#k: parser_kind)
+  (#t: Type)
+  (#p: parser k t)
+  (#vp: v base k t)
+  (#vres: AP.v base byte)
+  (a: byte_array base)
+  (va: AP.v base byte)
+  (res: byte_array base)
+: STGhost unit opened
+    (aparse p a vp `star` AP.arrayptr res vres)
+    (fun _ -> AP.arrayptr a va)
+    (
+      let consumed = AP.length (array_of vp) in
+      k.parser_kind_subkind == Some ParserStrong /\
+      AP.merge_into (array_of vp) (AP.array_of vres) (AP.array_of va) /\
+      consumed <= AP.length (AP.array_of va) /\
+      parse' p (AP.contents_of' va) == Some (vp.contents, consumed) /\
+      AP.contents_of' vres == AP.seq_slice (AP.contents_of' va) consumed (AP.length (AP.array_of va))
+    )
+    (fun _ -> True)
+= let va' = unpeek_strong' a res in
+  parse_injective p (AP.contents_of' va) (AP.contents_of' va');
+  Seq.lemma_split (AP.contents_of' va) (AP.length (array_of vp));
+  Seq.lemma_split (AP.contents_of' va') (AP.length (array_of vp));
+  rewrite
+    (AP.arrayptr a va')
+    (AP.arrayptr a va)
+
 let peek_consumes_all
   (#opened: _)
   (#base: Type)
@@ -264,3 +248,17 @@ let peek_consumes_all
 =
   parser_kind_prop_equiv k p;
   intro_aparse p a
+
+let leaf_reader
+  (#k: parser_kind)
+  (#t: Type)
+  (p: parser k t)
+: Tot Type
+= (#base: _) ->
+  (#va: _) ->
+  (a: byte_array base) ->
+  ST t
+    (aparse p a va)
+    (fun _ -> aparse p a va)
+    True
+    (fun res -> res == va.contents)
